theories/examples/authentikit_susp_security.v
@@ -4,6 +4,7 @@ From auth.heap_lang Require Import gen_weakestpre.
 From auth.heap_lang.lib Require Import list map.
 From auth.examples Require Export authentikit_susp authentikit_base_susp_security.
 From iris.base_logic.lib Require Export na_invariants.
+From iris.algebra Require Import auth agree numbers.
 
 (* Class tableG (Σ: gFunctors) := {
   tableG_na_invG :: na_invG Σ;
@@ -14,9 +15,42 @@ Definition table_inv `{!invGS_gen hlc Σ} `{!tableG Σ} (N : namespace) (P : iPr
   na_inv tableG_name N P.
 Definition table_tok `{!invGS_gen hlc Σ} `{!tableG Σ} (E : coPset) :=
   na_own tableG_name E. *)
+
+Definition msizeUR := authUR natUR.
+Class msizeG Σ := MsizeG { msize_inG :> inG Σ msizeUR; msizeG_name : gname }.
+
+Definition idcntrUR := authUR nat.
+Class idcntrG Σ := IdcntrG { idcntr_inG :> inG Σ idcntrUR; idcntrG_name : gname }.
+
+Lemma msize_alloc `{inG Σ msizeUR} :
+  ⊢ |==> ∃ _ : msizeG Σ,
+      (own msizeG_name (●{DfracOwn (1/2)} 0) ∗
+         own msizeG_name (●{DfracOwn (1/2)} 0) ∗ own msizeG_name (◯ 0))%I.
+Proof.
+  iMod (own_alloc (● 0 ⋅ ◯ 0)) as (γ) "[Hauth Hfrag]"; [admit|].
+  set (H1 := MsizeG _ _ γ).
+  iExists _. iDestruct "Hauth" as "[$ $]".
+  by iFrame.
+Admitted.
+
+Lemma idcntr_alloc `{inG Σ idcntrUR} :
+  ⊢ |==> ∃ _ : idcntrG Σ, (own idcntrG_name (●{DfracOwn (1/2)} 0) ∗ own idcntrG_name (●{DfracOwn (1/2)} 0))%I.
+Proof.
+  iMod (own_alloc (● 0 ⋅ ◯ 0)) as (γ) "[Hauth _]"; [admit|].
+  set (H1 := IdcntrG _ _ γ).
+  iExists _.
+  by iDestruct "Hauth" as "[$ $]".
+Admitted.
+
+Lemma state_alloc `{inG Σ stateUR} :
+  ⊢ |==> ∃ _ : stateG Σ, (own stateG_name (● (∅, ∅)))%I.
+Proof.
+  iMod (own_alloc ((● (∅, ∅)) : stateUR)) as (γ) "Hst"; [admit|].
+  by iExists (StateG _ _ γ).
+Admitted.
   
 Section proof.
-  Context `{!stateG Σ, !authG Σ, !seqG Σ}.
+  Context `{!msizeG Σ, !idcntrG Σ, !stateG Σ, !authG Σ, !seqG Σ}.
 
   Definition authBaseN : namespace := nroot .@ "susp_ver".
   Definition authN (v : val) : namespace := authBaseN .@ v.
@@ -26,6 +60,13 @@ Section proof.
   Definition tableLocN (susp : val) : namespace := tableLocSet .@ susp.
 
   Definition lrel_auth := lrel_auth authBaseN.
+
+  Definition msize_auth (n : nat) : iProp Σ :=
+    own msizeG_name (●{DfracOwn (1/2)} n) ∗ own msizeG_name (◯ n).
+  Definition msize_frag (n : nat) : iProp Σ :=
+    own msizeG_name (●{DfracOwn (1/2)} n).
+
+  Definition idcntr_frag (n : nat) := own idcntrG_name (●{DfracOwn (1/2)} n).
 
   (* Definition proph_type : Type := nat * option unit.
 
@@ -158,16 +199,18 @@ Section proof.
                                                 finish_spec2 finish x a aᵥ aᵢ ser A))).
       
   Definition is_susp_table (l : loc) : iProp Σ :=
-    ∃ (d : val) (m : gmap val val),  l ↦ d ∗ ⌜is_map d m⌝ ∗ susp_big_sep m.
+    ∃ (d : val) (m : gmap val val) (s c : nat),
+      l ↦ d ∗ ⌜is_map d m s⌝ ∗ susp_big_sep m ∗ msize_auth s ∗
+        idcntr_frag c ∗ (∀ (id : nat), ⌜id ≥ c → m !! #id = None⌝).
 
   Definition in_susp_table (l : loc) (id : nat) : iProp Σ :=
-    ∃ (d v : val) (m : gmap val val),
-      is_susp_table l -∗ l ↦ d ∗ ⌜is_map d m⌝
+    ∃ (d v : val) (m : gmap val val) (s : nat),
+      is_susp_table l -∗ l ↦ d ∗ ⌜is_map d m s⌝
       -∗ is_susp_table l ∗ ⌜m !! #id = Some v⌝.
 
   Definition not_in_susp_table (l : loc) (id : nat) : iProp Σ :=
-    ∃ (d : val) (m : gmap val val),
-      is_susp_table l -∗ l ↦ d ∗ ⌜is_map d m⌝
+    ∃ (d : val) (m : gmap val val) (s : nat),
+      is_susp_table l -∗ l ↦ d ∗ ⌜is_map d m s⌝
       -∗ is_susp_table l ∗ ⌜m !! #id = None⌝.
 
   Definition inv_susp_table (l: loc) := seq_inv tableN (is_susp_table l).
@@ -180,38 +223,46 @@ Section proof.
                          (∀ id', lm !! l = Some id' → id ≠ id'))).
   
   Definition global_state (cnt : nat) (m : mapUR) (lm : locPidMapUR) : iProp Σ :=
-    own stateG_name (● (MaxNat (cnt-1), m, lm)) ∗
+    own stateG_name (● (m, lm)) ∗ idcntr_frag cnt ∗
       ⌜count_inv cnt m lm⌝ ∗
       (∀ (id : nat) (x vᵥ : val) (l : loc) (t : evi_type),
-          ⌜m !! id = Some (to_agree (t, x, vᵥ, (None : option loc), true))⌝ ∗
+          ⌜m !! id = Some (to_agree (t, x, vᵥ, (None : option loc), true))⌝ -∗
             (in_susp_table l id ∨ (not_in_susp_table l id ∗ val_eq t x vᵥ))).
   
-  Definition empty_state n : prodUR (prodUR max_natUR mapUR) locPidMapUR := (MaxNat n, ∅, ∅).
-  
-  Lemma global_state_update_empty E (cnt : nat) (m : mapUR) (lm : locPidMapUR) :
-    global_state cnt m lm ={E}=∗ global_state (cnt + 1) m lm.
+  Definition empty_state : prodUR mapUR locPidMapUR := (∅, ∅).
+
+  Lemma init_global_state :
+    idcntr_frag 0 ==∗ global_state 0 ∅ ∅.
   Proof.
-    iIntros "(Hproph & %Hcntinv & Hseminv)".
-    iMod ((own_update
-             stateG_name
-             (● (MaxNat (cnt-1), m, lm))
-             (● (MaxNat cnt, m, lm) ⋅ ◯ (empty_state cnt) ))
-           with "Hproph") as "Hproph".
-    { apply (auth_update _ (empty_state 0) _ _).
-      do 2 apply prod_local_update_1.
-      apply max_nat_local_update.
-      simpl. lia. }
-    iPoseProof (own_op with "Hproph") as "[Hproph _]".
-    iModIntro. rewrite /global_state.
-    rewrite Nat.add_sub. iFrame. iPureIntro.
-    intros id H. apply Hcntinv. lia.
-  Qed.
+    iIntros "Hfrag".
+    iFrame.
+    iMod state_alloc as (γs) "Hst".
+
+    iModIntro. iSplitL; [admit|].
+    iSplit.
+    { iPureIntro. intros ??. split; first done.
+      intros ?. by left. }
+    iIntros (??????). done.
+  Admitted.
+  
+  Lemma global_state_update_empty (cnt : nat) (m : mapUR) (lm : locPidMapUR) :
+    global_state cnt m lm ∗ idcntr_frag cnt ==∗ global_state (cnt+1) m lm ∗ idcntr_frag (cnt+1).
+  Proof.
+    iIntros "((Hst & Hcntfrag & %Hcntinv & Hseminv) & Hcntauth)".
+    
+    iCombine "Hcntauth Hcntfrag" as "Hfull".
+    iMod (own_update with "Hfull") as "[Hfull _]".
+    { apply (auth_update _ 0 (cnt+1) 1).
+      apply (nat_local_update _ _ (cnt+1)).
+      lia. }
+
+  Admitted.
 
   Definition singleton_map (id : nat) (t : evi_type) (x vᵥ : val) (so : option loc) (b : bool) : mapUR :=
     {[ id := to_agree (t, x, vᵥ, so, b) ]}.
 
   Definition single_instance_frag (id : nat) (t : evi_type) (x vᵥ : val) (so : option loc) (b : bool) : stateUR :=
-    ◯ (MaxNat id, singleton_map id t x vᵥ so b, if so is Some s then {[ s := id ]} else ∅).
+    ◯ (singleton_map id t x vᵥ so b, if so is Some s then {[ s := id ]} else ∅).
 
   Definition updated_map (m : mapUR) (id : nat) (t : evi_type) (x vᵥ : val) (so : option loc) (b : bool) : mapUR :=
     <[ id := to_agree (t, x, vᵥ, so, b) ]> m.
@@ -219,27 +270,38 @@ Section proof.
   Definition updated_loc_map (m : locPidMapUR) (so : option loc) (id : nat) : locPidMapUR :=
     if so is Some s then <[ s := id ]> m else m.
 
-  Lemma global_state_update_singleton E (cnt : nat) (m : mapUR) (lm : locPidMapUR) (t : evi_type) (x vᵥ : val) (so : option loc) (b : bool) :
-    global_state cnt m lm
-    ={E}=∗ global_state (cnt + 1) (updated_map m cnt t x vᵥ so b) (updated_loc_map lm so cnt) ∗ single_instance cnt t x vᵥ so b.
+  Lemma global_state_update_singleton (cnt : nat) (m : mapUR) (lm : locPidMapUR) (t : evi_type) (x vᵥ : val) (so : option loc) (b : bool) :
+    global_state cnt m lm ∗ idcntr_frag cnt
+    ==∗ global_state (cnt + 1) (updated_map m cnt t x vᵥ so b) (updated_loc_map lm so cnt) ∗ single_instance cnt t x vᵥ so b ∗ idcntr_frag (cnt + 1).
   Proof.
-    iIntros "(Hproph & %Hcntinv & Hseminv)".
+    iIntros "((Hst & Hcntfrag & %Hcntinv & Hseminv) & Hcntauth)".
     iMod ((own_update
              stateG_name
-             (● (MaxNat (cnt-1), m, lm))
-             (● (MaxNat cnt, updated_map m cnt t x vᵥ so b, updated_loc_map lm so cnt) ⋅ single_instance_frag cnt t x vᵥ so b))
-           with "Hproph") as "Hproph".
-    { apply (auth_update _ (empty_state 0) _ _).
+             (● (m, lm))
+             (● (updated_map m cnt t x vᵥ so b, updated_loc_map lm so cnt) ⋅ single_instance_frag cnt t x vᵥ so b))
+           with "Hst") as "Hst".
+    { apply (auth_update _ empty_state _ _).
       apply prod_local_update; simpl.
-      { apply prod_local_update; simpl.
-        { apply max_nat_local_update. simpl. lia. }
-        apply gmap.alloc_local_update; last done.
+      { apply gmap.alloc_local_update; last done.
         apply Hcntinv. lia. }
       destruct so; last done.
       admit. }
-    iPoseProof (own_op with "Hproph") as "[Hproph Hfrag]".
-    iModIntro. rewrite /global_state.
-    rewrite Nat.add_sub. iFrame. iSplitR "Hseminv".
+    iPoseProof (own_op with "Hst") as "[Hst Hfrag]".
+
+    iCombine "Hcntauth Hcntfrag" as "Hfull".
+    iMod (own_update with "Hfull") as "[Hfull _]".
+    { apply (auth_update _ 0 (cnt+1) 1).
+      apply (nat_local_update _ _ (cnt+1)).
+      lia. }
+
+    iAssert (idcntr_frag (cnt + 1) ∗ idcntr_frag (cnt + 1))%I with "[Hfull]" as "[H1 H2]".
+    { admit. }
+
+    iModIntro.
+    iSplitR "H2 Hfrag"; [|iFrame].
+
+    rewrite /global_state.
+    iFrame. iSplitR "Hseminv".
     iPureIntro.
     { intros id H. rewrite /updated_map.
       rewrite lookup_insert_None.
@@ -248,10 +310,46 @@ Section proof.
       apply Hcntinv. lia. }
     iIntros (?????).
     iSpecialize ("Hseminv" $! id x0 vᵥ0 l t0) as #.
-    iDestruct "Hseminv" as "[%Hseminv $]".
-    iPureIntro. unfold updated_map.
+    iIntros (?). iApply "Hseminv".
   Admitted.
-  
+
+  Lemma msize_agree (s s' : nat) :
+    msize_auth s ∗ msize_frag s' -∗ ⌜s = s'⌝ ∗ msize_auth s ∗ msize_frag s'.
+  Proof.
+    iIntros "[[Hauth1 Hfrag] Hauth2]".
+    iCombine "Hauth1 Hauth2" as "Hauth".
+    iDestruct (own_valid with "Hauth") as "%H".
+    move: H => /auth_auth_dfrac_op_inv ->.
+
+    iDestruct "Hauth" as "[Hauth1 Hauth2]". by iFrame.
+  Qed.
+
+  Lemma msize_update (s s': nat) :
+    msize_auth s ∗ msize_frag s ==∗ msize_auth s' ∗ msize_frag s'.
+  Proof.
+    iIntros "[[Hauth1 Hfrag] Hauth2]".
+    iCombine "Hauth1 Hauth2" as "Hauth".
+    iMod (own_update_2 with "Hauth Hfrag") as "[Hauth Hfrag]".
+    { apply (auth_update s s s' s').
+      apply nat_local_update. lia. }
+
+    iDestruct "Hauth" as "[Hauth1 Hauth2]".
+    by iFrame.
+  Qed.
+    
+  Lemma idcntr_agree (cnt cnt' : nat) :
+    ∀ m lm, global_state cnt m lm ∗ idcntr_frag cnt'
+            -∗ ⌜cnt = cnt'⌝ ∗ global_state cnt m lm ∗ idcntr_frag cnt.
+  Proof.
+    iIntros (??) "[(? & Hcntfrag & ?) Hidauth]".
+    iCombine "Hcntfrag Hidauth" as "Hfull".
+    iDestruct (own_valid with "Hfull") as "%H".
+    move: H => /auth_auth_dfrac_op_inv H.
+    rewrite H.
+
+    iDestruct "Hfull" as "[Hcntfrag Hidauth]".
+    by iFrame.
+  Qed.
     
 (*  Definition proph_list (vs : val) : iProp Σ :=
     ∃ (m: gmap int proph_id),
@@ -543,22 +641,21 @@ Section proof.
     LRel (λ v1 a2, ∃ a1 prf1 counter, ⌜v1 = (prf1, a1)%V⌝ ∗ is_proof_state prf1 counter ∗ A a1 a2)%I.
 
   Definition lrel_auth_comp_post_bad (A : lrel Σ) : lrel Σ :=
-    LRel (λ v1 v2, ∃ t a1 prf1 x counter,
-          ⌜v1 = (prf1, x)%V⌝ ∗ is_proof_state prf1 counter ∗ s_valid_val authBaseN t x ∗
-            A a1 v2)%I.
+    LRel (λ v1 v2, ∃ a1 prf1 x counter,
+          ⌜v1 = (prf1, x)%V⌝ ∗ is_proof_state prf1 counter ∗ A a1 v2)%I.
 
   Definition lrel_auth_comp' (A : lrel Σ) : lrel Σ := LRel (λ v1 v2,
-    ∀ t K (w w' : val) m lm (cntr : nat),
+    ∀ t K (w w' : val) m lm (cntr l1 : nat),
       {{{ spec_ideal t (fill K (v2 w')) ∗ seq_tok ⊤ ∗ is_proof_state w cntr ∗
-            global_state cntr m lm }}}
+            global_state cntr m lm ∗ msize_frag l1 }}}
         v1 w
       {{{ (o1 : option val), RET $o1;
           seq_tok ⊤ ∗
             if o1 is Some w1 then
-              ∃ (w2 a prfst prf : val) (cntr' : nat) m' lm',
+              ∃ (w2 a prfst prf : val) (cntr' l2 : nat) m' lm',
                 spec_ideal t (fill K w2) ∗ ⌜w1 = (prfst, a)%V ∧ prfst = (prf, #cntr')%V⌝ ∗
-                           global_state cntr' m' lm' ∗
-                           (lrel_auth_comp_post A w1 w2 ∨ lrel_auth_comp_post_bad A w1 w2)
+                  global_state cntr' m' lm' ∗ msize_frag l2 ∗
+                  ((⌜l2 = 0⌝ ∗ lrel_auth_comp_post A w1 w2) ∨ (⌜l2 ≠ 0⌝ ∗ lrel_auth_comp_post_bad A w1 w2))
             else True }}})%I.
 
   (* Definition lrel_auth_comp_bad : lrel Σ := LRel (λ v1 v2,
@@ -576,11 +673,11 @@ Section proof.
   Program Definition lrel_auth_comp : kindO Σ (⋆ ⇒ ⋆)%kind := λne A, lrel_auth_comp' A.
   Next Obligation.
     intros ??? ???. rewrite /lrel_car /=.
-    do 43 f_equiv; solve_proper.
+    do 49 f_equiv; solve_proper.
   Qed.
 
   Definition lrel_hash_fail_option' (A : lrel Σ) : lrel Σ := LRel (λ v1 v2,
-    (A v1 v2 ∨ (∃ t x, A x v2 ∗ s_valid_val authBaseN t v1)))%I.
+    (A v1 v2 ∨ (∃ x, A x v2)))%I.
 
   Program Definition lrel_hash_fail_option : kindO Σ (⋆ ⇒ ⋆)%kind := λne A, lrel_hash_fail_option' A.
   Next Obligation.
@@ -603,17 +700,21 @@ Section proof.
     i_pures; wp_pures.
     iModIntro. iFrame. clear.
     interp_unfold!.
-    iIntros (??????? Ψ) "!# (Hi & Htok & % & Hst) HΨ".
+    iIntros (???????? Ψ) "!# (Hi & Htok & % & Hst & Hs) HΨ".
     simpl in H. destruct H as (? & -> & Hp).
     i_pures; wp_pures.
     iModIntro. iApply ("HΨ" $! (Some _)).
     iFrame "Htok".
     iExists _, _, _, _. iFrame. iSplit; first done.
-    iLeft. iExists _, _.
-    interp_unfold in "HA".
-    iFrame "HA".
-    iExists _. iSplit; [done|]. rewrite /is_proof_state.
-    eauto.
+    destruct (decide (l1 = 0)); iFrame "%".
+    - iLeft. iExists _, _.
+      interp_unfold in "HA".
+      iFrame "HA".
+      iExists _. iSplit; [done|]. rewrite /is_proof_state.
+      eauto.
+    - iRight. do 4 iExists _.
+      interp_unfold in "HA".
+      iFrame "HA". done.
   Qed.
 
   Lemma refines_auth_bind Θ (Δ : ctxO Σ Θ) :
@@ -639,15 +740,15 @@ Section proof.
     iModIntro. iFrame. clear.
     interp_unfold!.
     interp_unfold in "HmA".
-    iIntros (u1 u2 ????? Ψ) "!# (Hi & Htok & Hprf & Hst) HΨ".
+    iIntros (u1 u2 ?????? Ψ) "!# (Hi & Htok & Hprf & Hst & Hs) HΨ".
     i_pures; wp_pures.
     i_bind (v2 _)%I; wp_bind (v1 _)%I.
-    wp_apply ("HmA" with "[$Hi $Htok $Hprf $Hst]").
+    wp_apply ("HmA" with "[$Hi $Htok $Hprf $Hst $Hs]").
     iIntros (o) "[Htok Ho]".
     destruct o; last first.
     { wp_pures. iApply ("HΨ" $! None). by iFrame. }
-    iDestruct "Ho" as (???????) "(Hi & %H & Hst & [H|H])".
-    + iDestruct "H" as (a1 a2 ? ->) "[#Hprf #HA]".
+    iDestruct "Ho" as (????????) "(Hi & %H & Hst & Hs & [H|H])".
+    + iDestruct "H" as (? a1 a2 ? ->) "[#Hprf #HA]".
       wp_pures.
       wp_bind (w1 _)%E; i_bind (w2 _ )%E.
       interp_unfold in "HmB".
@@ -658,21 +759,21 @@ Section proof.
       destruct! H. simplify_eq.
       iPoseProof "Hprf" as (??) "Hprf'". simplify_eq.
       interp_unfold in "H".
-      wp_apply ("H" with "[$Htok $Hi $Hprf $Hst]").
+      wp_apply ("H" with "[$Htok $Hi $Hprf $Hst $Hs]").
       iIntros (?) "(Htok & Ho) /=".
       iApply "HΨ". iFrame.
-    + iDestruct "H" as (????? ->) "(#Hprf & Hval & #HA)".
+    + iDestruct "H" as (????? ->) "(#Hprf & #HA)".
       wp_pures.
       wp_bind (w1 _)%E; i_bind (w2 _)%E.
       interp_unfold in "HmB".
-      iSpecialize ("HmB" with "[Hval] [$Hi $Htok]").
+      iSpecialize ("HmB" with "[HA] [$Hi $Htok]").
       { interp_unfold!. iRight. iFrame "# ∗". }
       wp_apply (wp_wand with "HmB").
       iIntros (v) "(% & Hi & H & Htok) /=".
       interp_unfold in "H".
       destruct! H. simplify_eq.
       iPoseProof "Hprf" as (??) "Hprf'". simplify_eq.
-      wp_apply ("H" with "[$Htok $Hi $Hprf $Hst]").
+      wp_apply ("H" with "[$Htok $Hi $Hprf $Hst $Hs]").
       iIntros (?) "(Htok & Ho) /=".
       iApply "HΨ". iFrame.
   Qed.
@@ -700,13 +801,13 @@ Section proof.
     interp_unfold in "Hevi Hauth".
     iDestruct "Hauth" as "[(% & -> & Hauth)|->]"; wp_pures; last first.
     { iFrame. iModIntro.
-      interp_unfold!. iIntros (????????) "!# (Hi & Htok & Hproof & Hst) HΦ".
+      interp_unfold!. iIntros (?????????) "!# (Hi & Htok & Hproof & Hst & Hs) HΦ".
       wp_pures.
       iApply ("HΦ" $! None). by iFrame. }
         
     iDestruct "Hevi" as (tA' ??? ->) "(#Hser' & #Hser3 & #Hcount & #Hdeser & #Hrel & #Hcupd)".
     iFrame. iModIntro.
-    interp_unfold!. iIntros (????????) "!# (Hi & Htok & Hproof & Hst) HΦ".
+    interp_unfold!. iIntros (?????????) "!# (Hi & Htok & Hproof & Hst & Hs) HΦ".
     wp_pures. i_pures. iDestruct "Hproof" as (? -> ) "Hproof".
     wp_pures. iDestruct "Hproof" as "(% & %)".
     wp_apply gwp_list_head; [done| ].
@@ -742,58 +843,82 @@ Section proof.
         iNext. iIntros ([]) "(Htok & #HAfin)"; wp_pures; last first.
         { iApply ("HΦ" $! (None)). eauto. }
         wp_apply gwp_list_tail; [done|].
-        iIntros (vl Hl). wp_pures.
+        iIntros (vl Hl).
 
-        iMod (global_state_update_empty with "Hst") as "Hst".
+        iMod (na_inv_acc with "Htab Htok") as "(Htabo & Htok & Hclose_tab)"; [solve_ndisj|solve_ndisj|].
+        iDestruct "Htabo" as (????) "(Hl & >%Hm & Hbigsep & Hms & Hfrag & >%Hci)".
+        wp_pures.
+
+        iPoseProof (idcntr_agree with "[$Hst $Hfrag]") as (->) "[Hst Hfrag]".
+        iMod (global_state_update_empty with "[$Hst $Hfrag]") as "[Hst Hfrag]".
         
         iApply ("HΦ" $! (Some _)).
+        iMod ("Hclose_tab" with "[$Hl $Hbigsep $Htok $Hfrag $Hms]") as "Htok".
+        { iNext. iFrame "%". iIntros (id).
+          iPureIntro. intros ?.
+          apply Hci. lia. }
+        
         iFrame. iModIntro.
         iExists _, _, _.
         iSplit.
         { iPureIntro. split; first done.
           do 3 f_equal. lia. }
-        iLeft. iExists _, _, _.
-        iSplit; [done|]. iFrame "#".
-        iExists _. iSplit.
-        { iPureIntro. f_equal.
-          instantiate (1 := (S cntr)).
-          rewrite Nat2Z.inj_succ. done. }
-        iExists _. done.
+
+        destruct (decide (l1 = 0)); [iLeft|iRight]; (iSplit; [done|]).
+        { iExists _, _, _.
+          iSplit; [done|]. iFrame "#".
+          iExists _. iSplit.
+          { iPureIntro. f_equal.
+            instantiate (1 := (S c0)).
+            rewrite Nat2Z.inj_succ. done. }
+          iExists _. done. }
+        { do 4 iExists _.
+          iSplit; [done|]. iFrame "#".
+          iExists _. iSplit.
+          { iPureIntro. f_equal.
+            instantiate (1 := (S c0)).
+            rewrite Nat2Z.inj_succ. done. }
+          iExists _. done. }
 
       + iMod (na_inv_acc with "Htab Htok") as "(Htabo & Htok & Hclose_tab)"; [solve_ndisj|solve_ndisj|].
-        iDestruct "Htabo" as (??) "(Hl & Htabo)". wp_load.
-        iDestruct "Htabo" as (Hmap) "Hbigsep". wp_pures.
+        iDestruct "Htabo" as (????) "(Hl & >%Hm & Hbigsep & Hms & Hfrag & >%Hci)". wp_load.
 
-        iMod (global_state_update_singleton with "Hst") as "[Hst Hfrag]".
+        iPoseProof (idcntr_agree with "[$Hst $Hfrag]") as (->) "[Hst Hfrag]".
+        iPoseProof (msize_agree with "[$Hms $Hs]") as (<-) "[Hms Hs]".
+        iMod (global_state_update_singleton with "[$Hst $Hfrag]") as "(Hst & Hins & Hfrag)".
+
+        assert (m0 !! #c1 = None). { apply Hci. lia. }
+        wp_bind (map.map_insert _ _ _). wp_pures.
+        iApply (gwp_map_insert_none #c1 (#c0, finish)%V d m0 _ _ s); [done|done|done|].
         
-        wp_bind (map.map_insert _ _ _).
-        iApply (gwp_map_insert #cntr); [done|done|].
         iModIntro. iIntros (d') "%Hmap'". wp_store.
+        iMod (msize_update _ (s+1) with "[$Hms $Hs]") as "[Hms Hs]".
         wp_pures. wp_apply (gwp_list_tail with "[//]").
         iIntros "/=" (tl Htl). wp_pures.
-        iMod ("Hclose_tab" with "[$Hl Hbigsep $Htok Hfinish Hc Hfrag]") as "Htok".
-        { iFrame "%". iNext.
-          iApply (big_sepM_insert_2 with "[Hfinish Hc Hfrag]"); last done.
+        iMod ("Hclose_tab" with "[$Hl Hbigsep $Htok $Hfrag $Hms Hfinish Hc Hins]") as "Htok".
+        { iNext. iFrame "%". iSplit; last first.
+          { iIntros (id).
+            iPureIntro. intros ?. admit. }
+          iApply (big_sepM_insert_2 with "[Hfinish Hc Hins]"); last done.
           instantiate (1 := true).
           iFrame "∗ #". iExists _.
           assert (c0 > 0).
           { apply Nat.neq_0_lt_0. intros ->. by apply H0. }
           do 3 iExists _. repeat (try (iSplit; [done|])).
           iExists _. iLeft. iFrame. eauto. }
-        
-        iMod (deser_valid_weak with "Hval") as "Hval".
 
         iModIntro. iApply ("HΦ" $! (Some _)).
         iFrame. iExists _, _, _. iSplit.
         { iPureIntro. f_equal. split; first done.
           do 3 f_equal. lia. }
 
-        iRight. do 5 iExists _.
+        iRight. iSplit; [iPureIntro; lia|].        
+        do 4 iExists _.
         iSplit; first done.
         iFrame "# ∗".
         iExists _. iSplit.
         { iPureIntro. do 3 f_equal.
-          instantiate (1 := (S cntr)).
+          instantiate (1 := (S c1)).
           rewrite Nat2Z.inj_succ. done. }
         eauto.
 
@@ -831,64 +956,89 @@ Section proof.
           by iApply "HAfin". }
 
         wp_apply gwp_list_tail; [done|].
-        iIntros (vl Hl). wp_pures.
+        iIntros (vl Hl).
 
-        iMod (global_state_update_empty with "Hst") as "Hst".
+        iMod (na_inv_acc with "Htab Htok") as "(Htabo & Htok & Hclose_tab)"; [solve_ndisj|solve_ndisj|].
+        iDestruct "Htabo" as (????) "(Hl & >%Hm & Hbigsep & Hms & Hfrag & >%Hci)".
+        wp_pures.
+
+        iPoseProof (idcntr_agree with "[$Hst $Hfrag]") as (->) "[Hst Hfrag]".
+        iMod (global_state_update_empty with "[$Hst $Hfrag]") as "[Hst Hfrag]".
         
         iApply ("HΦ" $! (Some _)).
+        iMod ("Hclose_tab" with "[$Hl $Hbigsep $Htok $Hfrag $Hms]") as "Htok".
+        { iNext. iFrame "%". iIntros (id).
+          iPureIntro. intros ?.
+          apply Hci. lia. }
+        
         iFrame. iModIntro.
         iExists _, _, _.
         iSplit.
         { iPureIntro. split; first done.
           do 3 f_equal. lia. }
 
-        iLeft. iExists _, _, _.
-        iSplit; [done|]. iFrame "#".
-        iExists _. iSplit.
-        { iPureIntro. f_equal.
-          instantiate (1 := (S cntr)).
-          rewrite Nat2Z.inj_succ. done. }
-        iExists _. done.
+        destruct (decide (l1 = 0)); [iLeft|iRight]; (iSplit; [done|]).
+        { iExists _, _, _.
+          iSplit; [done|]. iFrame "#".
+          iExists _. iSplit.
+          { iPureIntro. f_equal.
+            instantiate (1 := (S c0)).
+            rewrite Nat2Z.inj_succ. done. }
+          iExists _. done. }
+        { do 4 iExists _.
+          iSplit; [done|]. iFrame "#".
+          iExists _. iSplit.
+          { iPureIntro. f_equal.
+            instantiate (1 := (S c0)).
+            rewrite Nat2Z.inj_succ. done. }
+          iExists _. done. }
 
       + iMod (na_inv_acc with "Htab Htok") as "(Htabo & Htok & Hclose_tab)"; [solve_ndisj|solve_ndisj|].
-        iDestruct "Htabo" as (??) "(Hl & Htabo)". wp_load.
-        iDestruct "Htabo" as (Hmap) "Hbigsep". wp_pures.
+        iDestruct "Htabo" as (????) "(Hl & >%Hm & Hbigsep & Hms & Hfrag & >%Hci)". wp_load.
 
-        iMod (global_state_update_singleton with "Hst") as "[Hst Hfrag]".
+        iPoseProof (idcntr_agree with "[$Hst $Hfrag]") as (->) "[Hst Hfrag]".
+        iPoseProof (msize_agree with "[$Hms $Hs]") as (<-) "[Hms Hs]".
+        iMod (global_state_update_singleton with "[$Hst $Hfrag]") as "(Hst & Hins & Hfrag)".
+
+        assert (m0 !! #c1 = None). { apply Hci. lia. }
+        wp_bind (map.map_insert _ _ _). wp_pures.
+        iApply (gwp_map_insert_none #c1 (#c0, finish)%V d m0 _ _ s); [done|done|done|].
         
-        wp_bind (map.map_insert _ _ _).
-        iApply (gwp_map_insert #cntr); [done|done|].
         iModIntro. iIntros (d') "%Hmap'". wp_store.
+        iMod (msize_update _ (s+1) with "[$Hms $Hs]") as "[Hms Hs]".
         wp_pures. wp_apply (gwp_list_tail with "[//]").
         iIntros "/=" (tl Htl). wp_pures.
-        iMod ("Hclose_tab" with "[$Hl Hbigsep $Htok Hfinish Hc Hfrag]") as "Htok".
-        { iFrame "%". iNext.
-          iApply (big_sepM_insert_2 with "[Hfinish Hc Hfrag]"); last done.
+        iMod ("Hclose_tab" with "[$Hl Hbigsep $Htok $Hfrag $Hms Hfinish Hc Hins]") as "Htok".
+        { iNext. iFrame "%". iSplit; last first.
+          { iIntros (id).
+            iPureIntro. intros ?. admit. }
+          iApply (big_sepM_insert_2 with "[Hfinish Hc Hins]"); last done.
           instantiate (1 := true).
           iFrame "∗ #". iExists _.
           assert (c0 > 0).
           { apply Nat.neq_0_lt_0. intros ->. by apply H0. }
           do 3 iExists _. repeat (try (iSplit; [done|])).
           iRight. iFrame. eauto. }
-        
-        iMod (deser_valid_weak authBaseN with "Hval") as "Hval".
 
         iMod ("Hclose" with "[$hashs1 Hval2 $Htok]") as "Htok".
-        { iNext. iLeft. iFrame "∗ #".  }
-
+        { iNext. iLeft. iFrame "∗ #". }
+        
         iModIntro. iApply ("HΦ" $! (Some _)).
+        
         iFrame. iExists _, _, _. iSplit.
         { iPureIntro. f_equal. split; first done.
           do 3 f_equal. lia. }
 
-        iRight. do 5 iExists _.
+        iRight. iSplit; [iPureIntro; lia|].        
+        do 4 iExists _.
         iSplit; first done.
         iFrame "# ∗".
         iExists _. iSplit.
         { iPureIntro. do 3 f_equal.
-          instantiate (1 := (S cntr)).
+          instantiate (1 := (S c1)).
           rewrite Nat2Z.inj_succ. done. }
-        eauto.
+        
+        iFrame "∗ %".
   Admitted.
         
   (* admit. (* What happens when we put finish in a map *)
@@ -1015,23 +1165,35 @@ Section proof.
     ⊢ REL v_Authenticable << i_Authenticable : ⟦ Authenticatable ⟧ (auth_ctx Δ).
   Proof.
     iIntros (??) "[Hi Htok]".
-    rewrite /i_Authenticable /v_Authenticable.
+    rewrite /i_Authenticable /v_Authenticable /v_Authenticable_run.
     wp_apply gwp_map_empty; [done|].
-    iIntros (d) "Hd".
-    i_bind (i_unauth)%V.
-    iMod (na_inv_alloc seqG_name ⊤ tableN (is_susp_table c) with "[$Hd $Hc]") as "#Htab".
-    { by iApply big_sepM_empty. }
-    i_bind _.
-    wp_pures. i_pures.
-    iPoseProof (refines_auth_unauth with "Htab [Hi $Htok]") as "Hwp".
+    iIntros (d) "Hd". wp_alloc l as "Hl". wp_pures.
+    
+    iMod msize_alloc as (γm) "[Hmfrag Hmauth]".
+    iMod idcntr_alloc as (γc) "[Hcauth Hcfrag]".
+    
+    iMod (na_inv_alloc seqG_name ⊤ tableN (is_susp_table l) with "[$Hd $Hl Hmauth Hcauth]") as "#Htab".
+    { iNext. iExists 0.
+      rewrite /msize_auth /idcntr_frag. iFrame.
+      iSplitR; [by iApply big_sepM_empty|].
+      iSplitL "Hmauth"; [admit|].
+      iSplitL "Hcauth"; [admit|].
+      iIntros (id). done. }
+    
+    iAssert (|={⊤}=> spec_ideal tᵢ (fill Kᵢ (i_Auth_auth, i_Auth_mu, i_Auth_pair, i_Auth_sum, i_Auth_string, i_Auth_int, i_auth, i_unauth)))%I with "[Hi]" as ">Hi"; [admit|].
+    
+    wp_rec. wp_pures.
+    wp_bind (v_unauth _).
+    i_bind (i_unauth).    
+    iPoseProof (refines_auth_unauth with "Htab [$Hi $Htok]") as "Hwp".
     wp_apply (wp_wand with "Hwp").
-    iIntros (?) "(% & Hi & #Hauth)".
+    iIntros (?) "(% & Hi & #Hauth & Htok)".
     iSimpl in "Hi".
     i_pures. wp_pures.
     iModIntro. iFrame.
     rewrite /Authenticatable.
     interp_unfold!.
-    iExists lrel_evidence.
+    iExists (lrel_evidence authBaseN).
     interp_unfold.
     iExists  _, _, _, _.
     do 2 (iSplit; [done|]).
@@ -1067,17 +1229,19 @@ Section proof.
     iSplit; last first.
     { iApply refines_Auth_mu. }
     iApply refines_Auth_auth.
-  Qed.
+  Admitted.
 
   Lemma refines_authentikit_func Θ (Δ : ctxO Σ Θ) :
-    ⊢ REL v_Authentikit << i_Authentikit : ⟦ Authentikit_func var1 var0 ⟧ (auth_ctx Δ).
+    ⊢ REL v_Authentikit << i_Authentikit : ⟦ Authentikit_func var2 var1 var0 ⟧ (auth_ctx Δ).
   Proof.
-    iIntros (??) "Hi".
+    iIntros (??) "[Hi Htok]".
     rewrite /i_Authentikit /v_Authentikit.
+    iAssert (|={⊤}=> spec_ideal tᵢ (fill Kᵢ (i_return, i_bind, i_Authenticable)))%I with "[Hi]" as ">Hi"; [admit|].
+    
     i_bind (i_Authenticable).
-    iPoseProof (refines_Authenticatable with "Hi") as "H".
+    iPoseProof (refines_Authenticatable with "[$Hi $Htok]") as "H".
     wp_apply (wp_wand with "H").
-    iIntros (?) "(% & Hv & #Hauth)".
+    iIntros (?) "(% & Hv & #Hauth & Htok)".
     iSimpl in "Hv".
     i_pures. wp_pures.
     iModIntro. iFrame.
@@ -1091,7 +1255,7 @@ Section proof.
     { iPoseProof refines_auth_return as "H". rewrite interp_unseal //. }
     iPoseProof refines_auth_bind as "?".
     rewrite interp_unseal //.
-  Qed.
+  Admitted.
 
   Lemma refines_authentikit Θ (Δ : ctxO Σ Θ) :
     ⊢ REL v_Authentikit << i_Authentikit : ⟦ Authentikit ⟧ Δ .
@@ -1099,68 +1263,185 @@ Section proof.
     iIntros (??) "Hi".
     iPoseProof (refines_authentikit_func with "Hi") as "H".
     wp_apply (wp_wand  with "H").
-    iIntros (?) "(% & $ & #Hauth)".
-    do 2 setoid_rewrite interp_exists_unfold.
-    by iExists lrel_auth, lrel_auth_comp.
+    iIntros (?) "(% & $ & #Hauth & Htok)".
+    do 3 setoid_rewrite interp_exists_unfold. iFrame.
+    by iExists lrel_hash_fail_option, lrel_auth, lrel_auth_comp.
   Qed.
 
   Lemma refines_run w (c1 c2 : expr) A :
-    seq_tok ⊤ -∗
     is_proof w -∗
     (REL c1 << c2 : lrel_auth_comp A) -∗
     refines_Some ⊤ (v_run #~ c1 w) (i_run #~ c2) A.
   Proof.
-    iIntros "Htok #Hprf Hc" (??) "Hi".
+    iIntros "#Hprf Hc".
+    iIntros (??) "[Hi Htok]".
     rewrite /v_run /i_run.
     wp_bind c1; i_bind c2.
-    iSpecialize ("Hc" with "Hi").
+    iSpecialize ("Hc" with "[$Hi $Htok]").
     wp_apply (wp_wand with "Hc").
-    iIntros (f1) "(%f2 & Hi & Hc) /=".
+    iIntros (f1) "(%f2 & Hi & Hc & Htok) /=".
+    rewrite /v_Authenticable_run.
+    rewrite /i_Authenticable /v_Authenticable /v_Authenticable_run.
+    wp_apply gwp_map_empty; [done|].
+    iIntros (d) "Hd". wp_alloc l as "Hl". wp_pures.
+    
+    iMod msize_alloc as (γm) "[Hmfrag Hmauth]".
+    iMod idcntr_alloc as (γc) "[Hcauth Hcfrag]".
+    
+    iMod (na_inv_alloc seqG_name ⊤ tableN (is_susp_table l) with "[$Hd $Hl Hmauth Hcauth]") as "#Htab".
+    { iNext. iExists 0.
+      rewrite /msize_auth /idcntr_frag. iFrame.
+      iSplitR; [by iApply big_sepM_empty|].
+      iSplitL "Hmauth"; [admit|].
+      iSplitL "Hcauth"; [admit|].
+      iIntros (id). done. }
+
+    wp_rec. wp_pures.
+    wp_rec. wp_pures.    
     wp_pures; i_pures.
-    wp_apply ("Hc" with "[$Hi $Htok $Hprf]").
+    iMod (init_global_state with "[Hcfrag]") as "Hst"; [admit|].
+    wp_apply ("Hc" with "[$Hi $Htok $Hprf Hmfrag Hst]").
+    { instantiate (4 := 0). iSplit. { iPureIntro. f_equal. }
+      rewrite /msize_frag. iFrame. admit. }
+
     iIntros (?) "(Htok & Ho)".
     destruct o1; last first.
-    { wp_pures. by iExists None. }
-    iDestruct "Ho" as (?) "[Hi H]".
-    wp_pures.
-    iDestruct "H" as (?? ->) "[% HA]".
-    wp_pures. iModIntro. iExists (Some _). eauto.
-  Qed.
+    { wp_pures. iExists None. by iFrame. }
+    
+    iMod (na_inv_acc with "Htab Htok") as "(Htabo & Htok & Hclose_tab)"; [solve_ndisj|solve_ndisj|].
+    iDestruct "Htabo" as (????) "(Hl & >%Hm & Hbigsep & >Hmauth & Hfrag & >%Hci)".
+    iDestruct "Ho" as (????????) "(Hi & % & Hst & Hmfrag & Hpost)".
+    iPoseProof (msize_agree with "[$Hmauth $Hmfrag]") as (->) "[Hmauth Hmfrag]".
+    wp_pures. wp_load.
+    wp_bind (map.map_is_empty _).
+    iApply (gwp_map_is_empty with "[]"); [done|].
+    iModIntro. iIntros (?) "%".
+    simpl in H0. subst.
+    iDestruct "Hpost" as "[[-> Hpost]|[% Hpost]]".
+    - wp_pures.
+      destruct! H. simplify_eq. wp_pures.
+      iMod ("Hclose_tab" with "[$Htok $Hbigsep $Hmauth $Hfrag $Hl]") as "Htok".
+      { iNext. iFrame "%". }
+      iModIntro. iExists (Some _).
+      iDestruct "Hpost" as (???) "(% & Hprf' & #HA)".
+      iFrame "∗". iSplit; first done. by simplify_eq.
+    - destruct l2; [done|]. wp_pures.
+      iMod ("Hclose_tab" with "[$Htok $Hbigsep $Hmauth $Hfrag $Hl]") as "Htok".
+      { iNext. iFrame "%". }
+      iModIntro. iExists None. by iFrame.
+  Admitted.
 
   Lemma refines_instantiate (c1 c2 : expr) (τ : type _ ⋆) :
-    (REL c1 << c2 : ⟦ ∀: ⋆ ⇒ ⋆; ⋆ ⇒ ⋆, Authentikit_func var1 var0 → var0 τ ⟧ ∅) -∗
-    REL c1 #~ #~ v_Authentikit
-     << c2 #~ #~ i_Authentikit : lrel_auth_comp (⟦ τ ⟧ (auth_ctx ∅)).
+    (REL c1 << c2 : ⟦ ∀: ⋆ ⇒ ⋆; ⋆ ⇒ ⋆; ⋆ ⇒ ⋆, Authentikit_func var2 var1 var0 → var0 τ ⟧ ∅) -∗
+    REL c1 #~ #~ #~ v_Authentikit
+     << c2 #~ #~ #~ i_Authentikit : lrel_auth_comp (⟦ τ ⟧ (auth_ctx ∅)).
   Proof.
-    iIntros "Hc" (??) "Hi".
+    iIntros "Hc" (??) "[Hi Htok]".
     wp_bind v_Authentikit. i_bind i_Authentikit.
-    iPoseProof (refines_authentikit_func with "Hi") as "H".
+    iPoseProof (refines_authentikit_func with "[$Hi $Htok]") as "H".
     wp_apply (wp_wand with "H").
-    iIntros (?) "(% & Hi & #Hauth)".
+    iIntros (?) "(% & Hi & #Hauth & Htok)".
     wp_bind c1; i_bind c2.
-    iSpecialize ("Hc" with "Hi").
+    iSpecialize ("Hc" with "[$Hi $Htok]").
     wp_apply (wp_wand with "Hc").
-    iIntros (v1) "(%v2 & Hi & Hcnt)".
-    iSpecialize ("Hcnt" $! lrel_auth with "[//]").
+    iIntros (v1) "(%v2 & Hi & Hcnt & Htok)".
+    iSpecialize ("Hcnt" $! lrel_hash_fail_option with "[//]").
     i_bind (v2 _).
-    iSpecialize ("Hcnt" with "Hi").
+    iSpecialize ("Hcnt" with "[$Hi $Htok]").
     wp_apply (wp_wand with "Hcnt").
-    iIntros (v1') "(%v2' & Hi & Hcnt)".
-    iSpecialize ("Hcnt" $! lrel_auth_comp with "[//]").
+    iIntros (v1') "(%v2' & Hi & Hcnt & Htok)".
+    iSpecialize ("Hcnt" $! lrel_auth with "[//]").
     i_bind (v2' _).
-    iSpecialize ("Hcnt" with "Hi").
+    iSpecialize ("Hcnt" with "[$Hi $Htok]").
     wp_apply (wp_wand with "Hcnt").
-    iIntros (v1'') "(%v2'' & Hi & Hcnt)".
+    iIntros (v1'') "(%v2'' & Hi & Hcnt & Htok)".
+    iSpecialize ("Hcnt" $! lrel_auth_comp with "[//]").
     i_bind (v2'' _).
-    interp_unfold! in "Hcnt".
-    iSpecialize ("Hcnt" with "[] Hi"); rewrite -!/interp; [done|].
+    iSpecialize ("Hcnt" with "[$Hi $Htok]").
     wp_apply (wp_wand with "Hcnt").
-    iIntros (v1''') "(%v2'''& Hi & Hcnt)".
+    iIntros (v1''') "(%v2''' & Hi & Hcnt & Htok)".
+    i_bind (v2''' _).
+    interp_unfold! in "Hcnt".
+    iSpecialize ("Hcnt" with "[] [$Hi $Htok]"); rewrite -!/interp; [done|].
+    wp_apply (wp_wand with "Hcnt").
+    iIntros (v1'''') "(%v2''''& Hi & Hcnt & Htok)".
     iEval (rewrite interp_app_unfold) in "Hcnt".
     interp_unfold in "Hcnt".
     iFrame.
   Qed.
 
 End proof.
+  
+Theorem authentikit_security Σ `{msizeG Σ, idcntrG Σ, stateG Σ, authPreG Σ, seqG Σ} (A : ∀ `{msizeG Σ, idcntrG Σ, stateG Σ, authG Σ, seqG Σ}, lrel Σ)
+  (φ : val → val → Prop) (cᵥ cᵢ : expr) (σ : state) (l : list string) (prf : val) :
+  (∀ `{msizeG Σ, idcntrG Σ, stateG Σ, authG Σ, seqG Σ}, ∀ vᵥ vᵢ, A vᵥ vᵢ -∗ ⌜φ vᵥ vᵢ⌝) →
+  (∀ `{msizeG Σ, idcntrG Σ, stateG Σ, authG Σ, seqG Σ}, ⊢ REL cᵥ << cᵢ : lrel_auth_comp A) →
+  is_list l prf →
+  adequate hash_collision NotStuck (v_run #~ cᵥ prf) σ
+    (λ vᵥ σᵥ, ∃ thpᵢ σᵢ vᵢ o,
+        vᵥ = $o ∧
+          if o is Some wᵥ then
+            (** a valid ideal execution *)
+            rtc erased_step ([i_run #~ cᵢ], σ) (of_val vᵢ :: thpᵢ, σᵢ) ∧
+              (** [φ] holds *)
+              φ wᵥ vᵢ
+          else True).
+Proof.
+  intros HA Hcomp Hprf.
+  eapply (heap_adequacy_strong Σ).
+  iIntros (Hinv) "_".
+  iMod (cfg_alloc (i_run #~ cᵢ) σ) as (Hcfgᵢ) "[Hauthᵢ Heᵢ]".
+  set (Hcfg := AuthG _ _ Hcfgᵢ).
+  iMod (inv_alloc specN _ (spec_inv ([(i_run #~ cᵢ)], σ)) with "[Hauthᵢ]") as "#Hcfg".
+  { iNext. iExists _, _. iFrame "# ∗ %". eauto. }
+  iAssert (spec_ctx) as "#Hctx"; [by iExists _|].
+  iMod na_alloc as (np) "Htok".
+  set (Hseq := Build_seqG _ _ np).
+
+  wp_apply wp_fupd.
+  wp_apply (wp_wand with "[-]").
+  { iPoseProof (refines_run (seqG0 := Hseq) prf with "[] []") as "Hrun".
+    - by iExists _.
+    - iApply Hcomp.
+    - iApply ("Hrun" $! empty_ectx with "[$Hctx $Heᵢ $Htok]"). }
+  iIntros (v) "(%o & -> & Htok & Ho)".
+  destruct o; last first.
+  { iIntros "!#" (????) "_". by iExists inhabitant, inhabitant, inhabitant, None. }
+  iDestruct "Ho" as "(%vᵢ & [_ Hi] & Hinterp) /=".
+
+  iDestruct (HA with "Hinterp") as %Hφ.
+  iInv specN as (tpᵢ σᵢ) ">(Hauthᵢ & %)" "Hclose".
+  iDestruct (cfg_auth_tpool_agree with "Hauthᵢ Hi") as %?.
+  destruct tpᵢ as [|? tpᵢ]; simplify_eq/=.
+  iMod ("Hclose" with "[-]") as "_".
+  { iExists (_ :: tpᵢ), σᵢ. iFrame "∗ % #". }
+  iModIntro.
+  iIntros (σᵥ ???) "(?&?&?&?& Hhashes)".
+  iIntros "!%". do 3 eexists; eexists (Some _). eauto.
+Qed.
+
+Theorem authentikit_security_syntactic (c : expr) (σ : state) (τ : type _ ⋆) prf (l : list string) :
+  EqType τ →
+  ε |ₜ ∅ ⊢ₜ c : (∀: ⋆ ⇒ ⋆; ⋆ ⇒ ⋆; ⋆ ⇒ ⋆, Authentikit_func var2 var1 var0 → var0 τ) →
+                is_list l prf →
+                adequate hash_collision NotStuck (v_run #~ (c #~ #~ #~ v_Authentikit) prf) σ
+                  (λ vᵥ σᵥ, ∃ thpᵢ σᵢ vᵢ o,
+                      vᵥ = $o ∧
+                        if o is Some wᵥ then
+                          (** a valid ideal execution *)
+                          rtc erased_step ([i_run #~ (c #~ #~ #~ i_Authentikit)], σ) (of_val vᵢ :: thpᵢ, σᵢ) ∧
+                            (** and they return the same value *)
+                            wᵥ = vᵢ
+                        else True).
+Proof.
+  intros Hτ Htyped Hprf.
+  set Σ := (#[authΣ; na_invΣ; GFunctor msizeUR; GFunctor idcntrUR; GFunctor stateUR]).
+  eapply (authentikit_security Σ (λ _ _ _ _ _, ⟦ τ ⟧ (auth_ctx ∅))); [| |done].
+  { iIntros (???????) "Hτ". by iDestruct (eq_type_sound with "Hτ") as %->. }
+  iIntros (?????).
+  iApply refines_instantiate.
+  by iApply refines_typed.
+Admitted.
+
 
              
